src/Ext/Expr.v
@@ -3,7 +3,6 @@ Require Export ExprCore.
 (*
 Require Export ExprT.
 Require Export ExprFacts.
-Require Export ExprProp.
 Require Export ExprLift.
 Require Export ExprSubst.
 Require Export ExprSimplify.
